simple_arm: update

s2n-bignum-examples/simple_arm.ml
@@ -1,17 +1,41 @@
 (****** A simple specification about program 'simple_arm.S' *******)
 
-needs "arm/proofs/base.ml";;
+(* If you are using HOL Light Online, this line is not necessary. *)
+(* needs "arm/proofs/base.ml";; *)
 
-(* save_literal_from_elf "bytelist.txt" "simple_arm.o";; *)
+let simple_arm_mc = new_definition `simple_arm_mc = [
+    word 0xe0; word 0x03; word 0x1f; word 0xaa; // arm_MOV X0 XZR
+    word 0x00; word 0x04; word 0x00; word 0x91; // arm_ADD X0 X0 (rvalue (word 1))
+    word 0x1f; word 0x0c; word 0x00; word 0xf1; // arm_CMP X0 (rvalue (word 3))
+    word 0xc1; word 0xff; word 0xff; word 0x54  // arm_BNE (word 2097144)
+  ]:((8)word)list`;;
+(* Or, you can read .o file and store the byte list as follows:
 let simple_arm_mc = define_assert_from_elf "simple_arm_mc" "simple_arm.o"
 [
   0xaa1f03e0;       (* arm_MOV X0 XZR *)
   0x91000400;       (* arm_ADD X0 X0 (rvalue (word 1)) *)
   0xf1000c1f;       (* arm_CMP X0 (rvalue (word 3)) *)
   0x54ffffc1        (* arm_BNE (word 2097144) *)
-];;
+];; *)
+
 let EXEC = ARM_MK_EXEC_RULE simple_arm_mc;;
 
+(*
+  In s2n-bignum, a specification (ensures) has three components:
+  1. precondition: assume that a program starts from some program state satisfying the critera
+  2. postcondition: the program must reach to a program state satisfying the criteria
+  3. frame: the start program state and end program state must satisfy this relation (e.g., only changes callee-save register)
+  In this file,
+  1. precondition is:
+    - the 'simple_arm' binary is loaded at some location in memory, say 'pc'
+    - the arm program counter register, PC, has value pc+4
+    - the arm register X0 has value 1
+  2. postcondition is:
+    - the arm program counter register, PC, has value pc+8 (meaning that one instruction has been executed)
+    - the arm register X0 has value 2
+  3. frame is:
+    - the register values of PC, X0 and flags must have been changed
+*)
 let SIMPLE_SPEC = prove(
   `!pc.
   ensures arm
@@ -35,3 +59,27 @@ let SIMPLE_SPEC = prove(
   ENSURES_FINAL_STATE_TAC THEN
   (* Some unproven parts can be proven using ASM_REWRITE_TAC[]. *)
   ASM_REWRITE_TAC[]);;
+
+(* If you want to explore the process line by line, follow here: *)
+g `!pc.
+  ensures arm
+    // Precondition
+    (\s. aligned_bytes_loaded s (word pc) simple_arm_mc /\
+         read PC s = word (pc+4) /\
+         read X0 s = word 1)
+    // Postcondition
+    (\s. read PC s = word (pc+8) /\
+         read X0 s = word 2)
+    // Registers (and memory locations) that may change after execution
+    (MAYCHANGE [PC;X0] ,, MAYCHANGE SOME_FLAGS)`;;
+(* Unravel ARM flag registers! *)
+e(REWRITE_TAC[SOME_FLAGS]);;
+e(REPEAT STRIP_TAC);;
+(* Start symbolic execution with state 's0' *)
+e(ENSURES_INIT_TAC "s0");;
+(* Symbolically run one instruction *)
+e(ARM_STEPS_TAC EXEC (1--1));;
+(* Try to prove the postcondition as much as possible *)
+e(ENSURES_FINAL_STATE_TAC);;
+(* Some unproven parts can be proven using ASM_REWRITE_TAC[]. *)
+e(ASM_REWRITE_TAC[]);;
